Update W12.dfy

Dafny/W12.dfy
@@ -1,3 +1,11 @@
+/** 
+
+Methods, Asserts, Pre/post conditions
+Termination, Inductive Datatypes
+
+Ref. Programs and Proofs, Chapter 1-4 */
+
+
 /* Method and assert statements */
 method Triple (x : int) returns (r : int){
     var y := 2 * x;
@@ -88,9 +96,9 @@ method ReconstructFromMaxSum(s: int, m: int) returns (x: int, y: int)
 }
 
 method TestMaxSum(x: int, y: int) {
-var m, s := MaxSum(x, y);
-var xx, yy := ReconstructFromMaxSum(s, m);
-assert (xx == x && yy == y) || (xx == y && yy == x);
+    var m, s := MaxSum(x, y);
+    var xx, yy := ReconstructFromMaxSum(s, m);
+    assert (xx == x && yy == y) || (xx == y && yy == x);
 }
 
 /** Functions in Dafny */
@@ -122,8 +130,7 @@ method Caller_Abs()
  * All statements which are used for specification purposes are called ghost statements.
  * They are ignored by the compiler.
  * Examples: Pre/post conditions, asserts, functions.
- * Variables can also be declared to be ghost, in which case they cannot be used in definition of
- normal variables.
+ * Variables can also be declared to be ghost, in which case they cannot be used in definition of normal variables.
 */
 
 method Triple_with_ghost (x : int) returns (r : int)
@@ -145,8 +152,7 @@ ghost method DoubleQuadruple(x:int) returns (a:int, b:int)
 /** 
 - Dafny proves total correctness, and hence verifies that every method/function terminates.
 - To help Dafny prove termination, the 'decreases' clause can be used.
-- Dafny will check that the parameter of the decreases clause reduces from the original call to the 
-recursive call.
+- Dafny will check that the parameter of the decreases clause reduces from the original call to the recursive call.
 - Note that the parameter of the decreases clause must remain non-negative in all calls.
  */
 
@@ -171,8 +177,7 @@ A binary relation > is well-founded if
 * > satisfies the descending chain condition: there is no infinite descending chain of values
 a0, a1, a2,... such that a0 > a1 > a2 > ... 
 
-Dafny allows the parameter of the decreases clause to have different types. It pre-defines a well-founded relation
-for different types:
+Dafny allows the parameter of the decreases clause to have different types. It pre-defines a well-founded relation for different types (here X is the decreases-parameter of the original call, and y is the decreases-parameter of the recursive call):
 
 type of X and y    |      X > y 
 ------------------------------------
@@ -180,6 +185,7 @@ bool                      X && !y
 int                       X > y && X >= 0
 real                      X - 1.0 >= y && X >= 0.9
 seq<T>                    y is a consecutive proper sub-sequence of X
+inductive datatypes       y is structurally included in X
 
 Dafny checks the above well-founded relations between the decreases paramter of the original call and the recursive call.
 */
@@ -216,5 +222,62 @@ decreases m, n
     Ack(m-1, Ack(m,n-1))
 }
 
+/** Inductive Datatypes */
+
 datatype BYTree = BlueLeaf | YellowLeaf | Node(BYTree, BYTree)
+
+function BlueCount(t: BYTree): nat {
+  match t
+  case BlueLeaf => 1
+  case YellowLeaf => 0
+  case Node(left, right) => BlueCount(left) + BlueCount(right)
+}
+
+function ReverseColors (t: BYTree): BYTree {
+  match t
+  case BlueLeaf => YellowLeaf
+  case YellowLeaf => BlueLeaf
+  case Node(left, right) => Node(ReverseColors(left), ReverseColors(right))
+}
+
+/** Discriminators and Destructors */
+
+predicate IsNode (t: BYTree) {
+  match t 
+  case Node(_,_) => true
+  case _ => false
+}
+
+/** Dafny pre-defines discriminators (such as the one shown above) for every constructor.
+For BYTree, the discriminators are BlueLeaf?, YellowLeaf?, Node?
+ */
+
+method discriminators_test() {
+  var a := Node(BlueLeaf,YellowLeaf);
+  var b := BlueLeaf;
+  assert(a.Node?);
+  assert(b.Node?);
+}
+
+function GetLeft(t: BYTree): BYTree
+  requires t.Node?
+{
+  match t
+  case Node(left, _ ) => left
+}
+
+/** Dafny pre-defines a destructor such as the one shown above to obtain parameters of a constructor */
+
+datatype BYTree_2 = BlueLeaf_2 | YellowLeaf_2 | Node_2(left: BYTree_2, right: BYTree_2)
+
+function BlueCount_2 (t: BYTree_2):nat{
+  if t.BlueLeaf_2? then 1
+  else if t.YellowLeaf_2? then 0 
+  else BlueCount_2(t.left) + BlueCount_2(t.right)
+}
+
+
+
+
+
 
